Making Reval compile.

low/Monads.v
@@ -1,10 +1,12 @@
 (** Monads.
 * Provides some model for the C memory and some monads to manipulate it easily. **)
 
-(** * A model for the C memory **)
-
-Require Export Rinternals TLC.LibHeap Shared.
+Set Implicit Arguments.
+Require Export String.
+Require Export RinternalsAux TLC.LibHeap Shared.
 Require Import TLC.LibStream.
+
+(** * A model for the C memory **)
 
 (** The global state of the C environment. In particular, it maps SEXP
   pointers to their corresponding expressions. **)
@@ -31,7 +33,7 @@ Definition alloc_SExp (S : state) (e : SExpRec) : state * nat.
 Defined.
 
 (** Writes a value in the state. Might return [None] if the cell is not already allocated. **)
-Definition write_SExp (S : state) (p : nat) (e : SExpRec) : option state.
+Definition write_SExp_nat (S : state) (p : nat) (e : SExpRec) : option state.
   refine (match read_option S p as r return r = _ -> _ with
           | None => fun _ => None
           | Some _ => fun Eq => Some {|
@@ -45,21 +47,30 @@ Definition write_SExp (S : state) (p : nat) (e : SExpRec) : option state.
   - apply* state_fresh_locations_different.
 Defined.
 
+Definition write_SExp (S : state) (p : SExpRec_pointer) (e : SExpRec) :=
+  match p with
+  | None => None
+  | Some p => write_SExp_nat S p e
+  end.
+
+Definition read_SExp_nat (S : state) (p : nat) : option SExpRec :=
+  read_option S p.
+
 (** Reads a value in the state. **)
 Definition read_SExp (S : state) (p : SExpRec_pointer) :=
   match p with
   | None => None
-  | Some p => read_option S p
+  | Some p => read_SExp_nat S p
   end.
 
 Lemma alloc_SExp_read_SExp : forall S S' e p,
   alloc_SExp S e = (S', p) ->
   read_SExp S' (Some p) = Some e.
-Proof. introv Eq. inverts Eq. simpl. rewrite~ read_option_write_same. Qed.
+Proof. introv Eq. inverts Eq. do 2 unfolds. simpl. rewrite~ read_option_write_same. Qed.
 
-Lemma destruct_write_SExp_None : forall (S : state) p e,
+Lemma destruct_write_SExp_nat_None : forall (S : state) p e,
   read_option S p = None ->
-  write_SExp S p e = None.
+  write_SExp_nat S p e = None.
 Proof.
   introv E. unfolds.
   asserts R: (forall T P (x : option T) (f1 : None = x -> P None) (f2 : forall v, Some v = x -> _)
@@ -75,13 +86,13 @@ Proof.
   + symmetry in E. lets R': (rm R) (read_option S p). erewrite (R' _ _ E). destruct~ E.
 Qed.
 
-Lemma destruct_write_SExp : forall (S : state) p e v,
+Lemma destruct_write_SExp_nat : forall (S : state) p e v,
   read_option S p = Some v ->
   exists S',
-    write_SExp S p e = Some S'
+    write_SExp_nat S p e = Some S'
     /\ (S' : heap _ _) = write S p e.
 Proof.
-  introv E. unfolds write_SExp.
+  introv E. unfolds write_SExp_nat.
   asserts R: (forall T T' (x : option T) (f1 : None = x -> T') (f2 : forall v, Some v = x -> T')
       v (H : Some v = x),
     match x as r return r = x -> T' with
@@ -94,50 +105,92 @@ Proof.
     eexists. splits~.
 Qed.
 
-Lemma write_SExp_read_SExp_same : forall S S' e p,
-  write_SExp S p e = Some S' ->
+Lemma write_SExp_nat_read_SExp_same : forall S S' e p,
+  write_SExp_nat S p e = Some S' ->
   read_SExp S' (Some p) = Some e.
 Proof.
   introv E. simpl. destruct (read_option S p) eqn: E'.
-  + forwards (S2&E1&E2): destruct_write_SExp E'.
-    rewrite E in E1. inverts E1. rewrite E2. rewrite~ read_option_write_same.
-  + forwards Eq: destruct_write_SExp_None E'. rewrite Eq in E. false*.
+  + forwards (S2&E1&E2): destruct_write_SExp_nat E'.
+    rewrite E in E1. inverts E1. unfolds. rewrite E2. rewrite~ read_option_write_same.
+  + forwards Eq: destruct_write_SExp_nat_None E'. rewrite Eq in E. false*.
+Qed.
+
+Lemma write_SExp_read_SExp_same : forall S S' e p,
+  write_SExp S p e = Some S' ->
+  read_SExp S' p = Some e.
+Proof. introv E. destruct p; tryfalse. applys~ write_SExp_nat_read_SExp_same E. Qed.
+
+Lemma write_SExp_nat_read_SExp : forall S S' e p p',
+  write_SExp_nat S p e = Some S' ->
+  p <> p' ->
+  read_SExp S' (Some p') = read_SExp S (Some p').
+Proof.
+  introv E D. simpl. destruct (read_option S p) eqn: E'.
+  + forwards (S2&E1&E2): destruct_write_SExp_nat E'.
+    rewrite E in E1. inverts E1. unfolds. rewrite E2. rewrite~ read_option_write.
+  + forwards Eq: destruct_write_SExp_nat_None E'. rewrite Eq in E. false*.
 Qed.
 
 Lemma write_SExp_read_SExp : forall S S' e p p',
   write_SExp S p e = Some S' ->
   p <> p' ->
-  read_SExp S' (Some p') = read_SExp S (Some p').
+  read_SExp S' p' = read_SExp S p'.
 Proof.
-  introv E D. simpl. destruct (read_option S p) eqn: E'.
-  + forwards (S2&E1&E2): destruct_write_SExp E'.
-    rewrite E in E1. inverts E1. rewrite E2. rewrite~ read_option_write.
-  + forwards Eq: destruct_write_SExp_None E'. rewrite Eq in E. false*.
+  introv E D. destruct p; tryfalse. destruct p'.
+  + applys~ write_SExp_nat_read_SExp E.
+  + reflexivity.
+Qed.
+
+Lemma read_SExp_write_SExp_nat : forall S e e' p,
+  read_SExp S (Some p) = Some e ->
+  exists S', write_SExp_nat S p e' = Some S'.
+Proof.
+  introv E. simpl in E. forwards (S'&E1&E2): destruct_write_SExp_nat E.
+  exists S'. rewrite~ E1.
 Qed.
 
 Lemma read_SExp_write_SExp : forall S e e' p,
-  read_SExp S (Some p) = Some e ->
+  read_SExp S p = Some e ->
   exists S', write_SExp S p e' = Some S'.
-Proof.
-  introv E. simpl in E. forwards (S'&E1&E2): destruct_write_SExp E.
-  exists S'. rewrite~ E1.
-Qed.
+Proof. introv E. destruct p; tryfalse. applys~ read_SExp_write_SExp_nat E. Qed.
 
 
 (** * Monads **)
 
-(* TODO: Define JSCest’s style out type. *)
+(** A monad type for results. **)
+Inductive result (A : Type) :=
+  | result_success : state -> A -> result A (** The program terminated in this state with this result. **)
+  | result_error : state -> string -> result A (** The program resulted in the following error (not meant to be caught). **)
+  | result_impossible : state -> string -> result A (** This result should never happen. We provide a string to help debugging. **)
+  | result_not_implemented : string -> result A (** This result relies on a feature not yet implemented. **)
+  | result_bottom : state -> result A (** We are out of fuel to compute anything. **)
+  .
+Arguments result_error [A].
+Arguments result_impossible [A].
+Arguments result_not_implemented [A].
+Arguments result_bottom [A].
 
-Definition if_defined (A B : Type) (o : option A) (f : A -> option B) : option B :=
+(** A precision about [result_not_implemented] and [result_error]:
+* if the C source code of R throw a not-implemented error, we consider
+* this as an error thrown in the original interpreter and use the
+* constructor [result_error].
+* We only throw [result_not_implemented] when our Coq code has not
+* implemented a behaviour of R. **)
+
+(** The monad for result. **)
+Definition if_success (A B : Type) (r : result A) (f : state -> A -> result B) : result B :=
+  match r with
+  | result_success S0 a => f S0 a
+  | result_error S0 s => result_error S0 s
+  | result_impossible S0 s => result_impossible S0 s
+  | result_not_implemented s => result_not_implemented s
+  | result_bottom S0 => result_bottom S0
+  end.
+
+(** As for [if_success], but from an option type. We suppose that the option type is defined. **)
+Definition if_defined (A B : Type) S (o : option A) (f : A -> result B) : result B :=
   match o with
-  | None => None
   | Some x => f x
+  | None => result_impossible S "[if_defined] got an undefined result."
   end.
-
-Definition if_returns (A B : Type) (o : option (state * A)) (f : state -> A -> option B) : option B :=
-  match o with
-  | None => None
-  | Some (S0, x) => f S0 x
-  end.
-
 
