low/Reval.v
@@ -2,25 +2,29 @@
 * Describes how R evaluates expressions.
 * The content of this file is the Coq equivalent of the file src/main/eval.c. **)
 
-Require Export Rinternals Monads.
+Set Implicit Arguments.
+Require Export Monads.
+
+(** * Global structure of the interpreter **)
 
 (** A structure to deal with infinite execution (which is not allowed in Coq). Inspired from JSCert. **)
 Record runs_type : Type := runs_type_intro {
-    runs_eval : state -> SExpRec_pointer -> SExpRec_pointer -> option (state * SExpRec_pointer)
+    runs_eval : state -> SExpRec_pointer -> SExpRec_pointer -> result SExpRec_pointer
   }.
 
 
-Definition forcePromise runs (S : state) (e : SExpRec_pointer) : option (state * SExpRec_pointer) :=
-  if_defined (read_SExp S e) (fun exp =>
-    if_defined (get_promSxp e) (fun p =>
+(** * Interpreter functions **)
+
+Definition forcePromise runs (S : state) (e : SExpRec_pointer) : result SExpRec_pointer :=
+  if_defined S (read_SExp S e) (fun exp =>
+    if_defined S (get_promSxp exp) (fun p =>
       If prom_value p = R_UnboundValue then
         runs_eval runs S (prom_expr p) (prom_env p)
-      else Some (S, e))).
-
+      else result_success S e)).
 
 (** The eval function of https://github.com/wch/r-source/blob/trunk/src/main/eval.c#L538 **)
-Definition eval runs (S : state) (e rho : SExpRec_pointer) : option (state * SExpRec_pointer) :=
-  if_defined (read_SExp S e) (fun exp =>
+Definition eval runs (S : state) (e rho : SExpRec_pointer) : result SExpRec_pointer :=
+  if_defined S (read_SExp S e) (fun exp =>
     match type exp with
     | NilSxp
     | ListSxp
@@ -39,9 +43,10 @@ Definition eval runs (S : state) (e rho : SExpRec_pointer) : option (state * SEx
     | ExtptrSxp
     | WeakrefSxp
     | ExprSxp =>
-      Some (write_SExp S (e set_named exp), e)
+      if_defined S (write_SExp S e (set_named exp)) (fun S =>
+        result_success S e)
     | _ =>
-      if_defined (read_SExp S rho) (fun env =>
+      if_defined S (read_SExp S rho) (fun env =>
         match type exp with
         | EnvSxp =>
           match type exp with
@@ -51,7 +56,7 @@ Definition eval runs (S : state) (e rho : SExpRec_pointer) : option (state * SEx
              * https://github.com/wch/r-source/blob/trunk/src/main/eval.c#L5966
              * for the evaluator.
              * We do not consider byte code for now in this formalisation. **)
-            None
+            result_not_implemented "[eval] byte code"
           | SymSxp =>
             (* TODO: https://github.com/wch/r-source/blob/trunk/src/main/eval.c#L626
              * I think that in essence, we are fetching the value of the symbol in the
@@ -59,40 +64,59 @@ Definition eval runs (S : state) (e rho : SExpRec_pointer) : option (state * SEx
             (** There is just a story about ddfindVar vs findVar which I don’t yet
              * understand (depending on the general purpose field). I need to investigate
              * about these two functions. **)
+            result_not_implemented "[eval] Symbols (TODO)"
           | PromSxp =>
-            if_defined (get_promSxp e) (fun p =>
-              Some (
-                If prom_value p = R_UnboundValue then
-                  forcePromise S e
-                else S,
-                p)
+            if_defined S (get_promSxp exp) (fun p =>
+              ifb prom_value p = R_UnboundValue then
+                if_success (forcePromise runs S e) (fun S e =>
+                  result_success S e)
+              else result_success S e)
           | LangSxp =>
-            if_defined (get_listSxp e) (fun l =>
-              if_defined (read_SExp S (list_carval l)) (fun car =>
-                if_returns
-                  (If type car = SymSxp then
+            if_defined S (get_listSxp exp) (fun l =>
+              let pcar := list_carval l in
+              if_defined S (read_SExp S pcar) (fun car =>
+                if_success
+                  (ifb type car = SymSxp then
                      (* TODO: findFun3 — in essence, this is just a variable look-up. *)
-                   else eval car rho) (fun S op =>
-                  if_defined (read_SExp S op) (fun opp =>
+                     result_not_implemented "[eval] findFun3 (TODO)"
+                   else runs_eval runs S pcar rho) (fun S op =>
+                  if_defined S (read_SExp S op) (fun opp =>
                     match type opp with
                     | SpecialSxp =>
                       (* TODO: This is basically a direct call to PRIMFUN. *)
+                      result_not_implemented "[eval] PRIMFUN (TODO)"
                     | BuiltinSxp =>
                       (* TODO: This is basically a call to PRIMFUN after evaluating the argument list. *)
+                      result_not_implemented "[eval] PRIMFUN after argument evaluation (TODO)"
                     | CloSxp =>
                       (* TODO: https://github.com/wch/r-source/blob/trunk/src/main/eval.c
                          applyClosure(e, op, promiseArgs(CDR(e), rho), rho, R_NilValue);
                        *)
-                    | _ => None
+                      result_not_implemented "[eval] applyClosure (TODO)"
+                    | _ => result_error S "[eval] Attempt to apply non-function."
                     end))))
-          | DotSxp =>
-            None
-          | _ => None
+          | DotSxp => result_error S "[eval] ‘...’ used in an incorrect context"
+          | _ => result_error S "[eval] Type unimplemented in the R source code."
           end
-        | _ => None
+        | _ => result_error S "[eval] ‘rho’ must be an environment."
         end)
     end).
 
 (** The property we want to eventually prove is that if [eval] returns
   a result, then the C function eval does similarly. **)
+
+
+(** * Closing the loop **)
+
+Fixpoint runs max_step : runs_type :=
+  match max_step with
+  | O => {|
+      runs_eval := fun S _ _ => result_bottom S
+    |}
+  | S max_step =>
+    let wrap {A : Type} (f : runs_type -> A) : A :=
+      f (runs max_step) in {|
+      runs_eval := wrap eval
+    |}
+  end.
 
