low/Rinternals.v
@@ -2,6 +2,8 @@
 * The types of this file exactly correspond to the types defined
 * in the R source file src/include/internals.h **)
 
+Set Implicit Arguments.
+
 (** * Types **)
 
 (** SEXPTYPE **)
@@ -159,53 +161,4 @@ Record Vector_SExpRec := {
     Vector_SExpRec_vecsxp :> VecSxp_struct
   }.
 *)
-
-
-(** * Accessors **)
-
-Definition get_primSxp e :=
-  match e with
-  | primSxp p => Some p
-  | _ => None
-  end.
-
-Definition get_listSxp e :=
-  match e with
-  | listSxp l => Some l
-  | _ => None
-  end.
-
-Definition get_envSxp e :=
-  match e with
-  | envSxp e => Some e
-  | _ => None
-  end.
-
-Definition get_cloSxp e :=
-  match e with
-  | cloSxp c => Some c
-  | _ => None
-  end.
-
-Definition get_promSxp e :=
-  match e with
-  | promSxp p => Some p
-  | _ => None
-  end.
-
-Definition set_named_sxpinfo i n :=
-  make_SxpInfo (type i) (obj i) n (mark i) (debug i) (trace i) (spare i) (gcgen i).
-
-Definition set_named_to e n :=
-  make_SExpRec
-    (let h := SExpRec_header e in
-     make_SExpRecHeader
-       (set_named_sxpinfo (sxpinfo h) n)
-       (attrib h)
-       (gengc_prev_node h)
-       (gengc_next_node h))
-    (SExpRec_data e).
-
-Definition set_named e :=
-  set_named_to e named_plural.
 
