low/RinternalsAux.v
@@ -1,0 +1,62 @@
+(** RinternalsAux.
+* Auxiliary definitions for the data structures defined in Rinternals. **)
+
+Set Implicit Arguments.
+Require Export Rinternals Shared.
+
+
+(** * Instances **)
+
+Instance SExpType_Comparable : Comparable SExpType.
+  prove_comparable_simple_inductive.
+Defined.
+
+
+(** * Accessors **)
+
+Definition get_primSxp e :=
+  match e with
+  | primSxp p => Some p
+  | _ => None
+  end.
+
+Definition get_listSxp e :=
+  match e with
+  | listSxp l => Some l
+  | _ => None
+  end.
+
+Definition get_envSxp e :=
+  match e with
+  | envSxp e => Some e
+  | _ => None
+  end.
+
+Definition get_cloSxp e :=
+  match e with
+  | cloSxp c => Some c
+  | _ => None
+  end.
+
+Definition get_promSxp e :=
+  match e with
+  | promSxp p => Some p
+  | _ => None
+  end.
+
+Definition set_named_sxpinfo i n :=
+  make_SxpInfo (type i) (obj i) n (mark i) (debug i) (trace i) (spare i) (gcgen i).
+
+Definition set_named_to e n :=
+  make_SExpRec
+    (let h := SExpRec_header e in
+     make_SExpRecHeader
+       (set_named_sxpinfo (sxpinfo h) n)
+       (attrib h)
+       (gengc_prev_node h)
+       (gengc_next_node h))
+    (SExpRec_data e).
+
+Definition set_named e :=
+  set_named_to e named_plural.
+
